Use Iris' iso_ofe infrastructure for types and seal off equiv and dist.

theories/typing/type.v
@@ -16,39 +16,49 @@ Definition lftE := ↑lftN.
 Definition lrustN := nroot .@ "lrust".
 Definition shrN  := lrustN .@ "shr".
 
+Definition thread_id := na_inv_pool_name.
+
+Record type `{typeG Σ} :=
+  { ty_size : nat;
+    ty_own : thread_id → list val → iProp Σ;
+    ty_shr : lft → thread_id → loc → iProp Σ;
+
+    ty_shr_persistent κ tid l : PersistentP (ty_shr κ tid l);
+
+    ty_size_eq tid vl : ty_own tid vl -∗ ⌜length vl = ty_size⌝;
+    (* The mask for starting the sharing does /not/ include the
+       namespace N, for allowing more flexibility for the user of
+       this type (typically for the [own] type). AFAIK, there is no
+       fundamental reason for this.
+       This should not be harmful, since sharing typically creates
+       invariants, which does not need the mask.  Moreover, it is
+       more consistent with thread-local tokens, which we do not
+       give any.
+
+       The lifetime token is needed (a) to make the definition of simple types
+       nicer (they would otherwise require a "∨ □|=>[†κ]"), and (b) so that
+       we can have emp == sum [].
+     *)
+    ty_share E κ l tid q : lftE ⊆ E →
+      lft_ctx -∗ &{κ} (l ↦∗: ty_own tid) -∗ q.[κ] ={E}=∗
+      ty_shr κ tid l ∗ q.[κ];
+    ty_shr_mono κ κ' tid l :
+      lft_ctx -∗ κ' ⊑ κ -∗ ty_shr κ tid l -∗ ty_shr κ' tid l
+  }.
+Existing Instance ty_shr_persistent.
+Instance: Params (@ty_size) 2.
+Instance: Params (@ty_own) 2.
+Instance: Params (@ty_shr) 2.
+
+Record simple_type `{typeG Σ} :=
+  { st_own : thread_id → list val → iProp Σ;
+    st_size_eq tid vl : st_own tid vl -∗ ⌜length vl = 1%nat⌝;
+    st_own_persistent tid vl : PersistentP (st_own tid vl) }.
+Existing Instance st_own_persistent.
+Instance: Params (@st_own) 2.
+
 Section type.
   Context `{typeG Σ}.
-
-  Definition thread_id := na_inv_pool_name.
-
-  Record type :=
-    { ty_size : nat;
-      ty_own : thread_id → list val → iProp Σ;
-      ty_shr : lft → thread_id → loc → iProp Σ;
-
-      ty_shr_persistent κ tid l : PersistentP (ty_shr κ tid l);
-
-      ty_size_eq tid vl : ty_own tid vl -∗ ⌜length vl = ty_size⌝;
-      (* The mask for starting the sharing does /not/ include the
-         namespace N, for allowing more flexibility for the user of
-         this type (typically for the [own] type). AFAIK, there is no
-         fundamental reason for this.
-         This should not be harmful, since sharing typically creates
-         invariants, which does not need the mask.  Moreover, it is
-         more consistent with thread-local tokens, which we do not
-         give any.
-
-         The lifetime token is needed (a) to make the definition of simple types
-         nicer (they would otherwise require a "∨ □|=>[†κ]"), and (b) so that
-         we can have emp == sum [].
-       *)
-      ty_share E κ l tid q : lftE ⊆ E →
-        lft_ctx -∗ &{κ} (l ↦∗: ty_own tid) -∗ q.[κ] ={E}=∗
-        ty_shr κ tid l ∗ q.[κ];
-      ty_shr_mono κ κ' tid l :
-        lft_ctx -∗ κ' ⊑ κ -∗ ty_shr κ tid l -∗ ty_shr κ' tid l
-    }.
-  Global Existing Instances ty_shr_persistent.
 
   (** Copy types *)
   Fixpoint shr_locsE (l : loc) (n : nat) : coPset :=
@@ -135,17 +145,6 @@ Section type.
     Sync ty → LstSync tys → LstSync (ty::tys) := List.Forall_cons _ _ _.
 
   (** Simple types *)
-  (* We are repeating the typeclass parameter here just to make sure
-     that simple_type does depend on it. Otherwise, the coercion defined
-     bellow will not be acceptable by Coq. *)
-  Record simple_type `{typeG Σ} :=
-    { st_own : thread_id → list val → iProp Σ;
-
-      st_size_eq tid vl : st_own tid vl -∗ ⌜length vl = 1%nat⌝;
-      st_own_persistent tid vl : PersistentP (st_own tid vl) }.
-
-  Global Existing Instance st_own_persistent.
-
   Program Definition ty_of_st (st : simple_type) : type :=
     {| ty_size := 1; ty_own := st.(st_own);
 
@@ -162,10 +161,9 @@ Section type.
     iMod (bor_exists with "LFT Hmt") as (vl) "Hmt". set_solver.
     iMod (bor_sep with "LFT Hmt") as "[Hmt Hown]". set_solver.
     iMod (bor_persistent with "LFT Hown") as "[Hown|#H†]". set_solver.
-    - iFrame "Hκ". iMod (bor_fracture with "LFT [Hmt]") as "Hfrac"; last first.
-      { iExists vl. iFrame. auto. }
-      done. set_solver.
-    - iExFalso. iApply (lft_tok_dead with "Hκ"). done.
+    - iFrame "Hκ".
+      iMod (bor_fracture with "LFT [Hmt]") as "Hfrac"; by eauto with iFrame.
+    - iExFalso. by iApply (lft_tok_dead with "Hκ").
   Qed.
   Next Obligation.
     intros st κ κ' tid l. iIntros "#LFT #Hord H".
@@ -175,25 +173,25 @@ Section type.
 
   Global Program Instance ty_of_st_copy st : Copy (ty_of_st st).
   Next Obligation.
-    intros st κ tid E ? l q ? HF. iIntros "#LFT #Hshr Htok Hlft".
+    iIntros (st κ tid E ? l q ? HF) "#LFT #Hshr Htok Hlft".
     iDestruct (na_own_acc with "Htok") as "[$ Htok]"; first set_solver+.
     iDestruct "Hshr" as (vl) "[Hf Hown]".
     iMod (frac_bor_acc with "LFT Hf Hlft") as (q') "[Hmt Hclose]"; first set_solver.
-    iModIntro. iExists _. iDestruct "Hmt" as "[Hmt1 Hmt2]". iSplitL "Hmt1".
-    - iNext. iExists _. by iFrame.
-    - iIntros "Htok2 Hmt1". iDestruct "Hmt1" as (vl') "[Hmt1 #Hown']".
-      iDestruct ("Htok" with "Htok2") as "$".
-      iAssert (▷ ⌜length vl = length vl'⌝)%I as ">%".
-      { iNext. iDestruct (st_size_eq with "Hown") as %->.
-        iDestruct (st_size_eq with "Hown'") as %->. done. }
-      iCombine "Hmt1" "Hmt2" as "Hmt". rewrite heap_mapsto_vec_op // Qp_div_2.
-      iDestruct "Hmt" as "[>% Hmt]". subst. by iApply "Hclose".
+    iModIntro. iExists _. iDestruct "Hmt" as "[Hmt1 Hmt2]".
+    iSplitL "Hmt1"; first by auto with iFrame.
+    iIntros "Htok2 Hmt1". iDestruct "Hmt1" as (vl') "[Hmt1 #Hown']".
+    iDestruct ("Htok" with "Htok2") as "$".
+    iAssert (▷ ⌜length vl = length vl'⌝)%I as ">%".
+    { iNext. iDestruct (st_size_eq with "Hown") as %->.
+      iDestruct (st_size_eq with "Hown'") as %->. done. }
+    iCombine "Hmt1" "Hmt2" as "Hmt". rewrite heap_mapsto_vec_op // Qp_div_2.
+    iDestruct "Hmt" as "[>% Hmt]". subst. by iApply "Hclose".
   Qed.
 
   Global Instance ty_of_st_sync st :
     Send (ty_of_st st) → Sync (ty_of_st st).
   Proof.
-    iIntros (Hsend κ tid1 tid2 l) "H". iDestruct "H" as (vl) "[Hm Hown]".
+    iIntros (Hsend κ tid1 tid2 l). iDestruct 1 as (vl) "[Hm Hown]".
     iExists vl. iFrame "Hm". iNext. by iApply Hsend.
   Qed.
 End type.
@@ -207,123 +205,119 @@ Bind Scope lrust_type_scope with type.
 Section ofe.
   Context `{typeG Σ}.
 
-  (* TODO: Use the ofe_iso infrastructure from Iris. *)
-  Section def.
-    Definition tuple_of_type (ty : type) : prodC (prodC _ _) _ :=
-      (ty.(ty_size),
-       Next (ty.(ty_own) : _ -c> _ -c> _),
-       ty.(ty_shr) :  _ -c> _ -c> _ -c> _).
+  Inductive type_equiv' (ty1 ty2 : type) : Prop :=
+    Type_equiv :
+      ty1.(ty_size) = ty2.(ty_size) →
+      (∀ tid vs, ty1.(ty_own) tid vs ≡ ty2.(ty_own) tid vs) →
+      (∀ κ tid l, ty1.(ty_shr) κ tid l ≡ ty2.(ty_shr) κ tid l) →
+      type_equiv' ty1 ty2.
+  Instance type_equiv : Equiv type := type_equiv'.
+  Inductive type_dist' (n : nat) (ty1 ty2 : type) : Prop :=
+    Type_dist :
+      ty1.(ty_size) = ty2.(ty_size) →
+      (∀ tid vs, dist_later n (ty1.(ty_own) tid vs) (ty2.(ty_own) tid vs)) →
+      (∀ κ tid l, ty1.(ty_shr) κ tid l ≡{n}≡ ty2.(ty_shr) κ tid l) →
+      type_dist' n ty1 ty2.
+  Instance type_dist : Dist type := type_dist'.
 
-    Instance type_equiv : Equiv type := λ ty1 ty2,
-       tuple_of_type ty1 ≡ tuple_of_type ty2.
-    Instance type_dist : Dist type := λ n ty1 ty2,
-       tuple_of_type ty1 ≡{n}≡ tuple_of_type ty2.
+  Let T := prodC
+    (prodC natC (thread_id -c> list val -c> laterC (iProp Σ)))
+    (lft -c> thread_id -c> loc -c> iProp Σ).
+  Let P (x : T) : Prop :=
+    (∀ κ tid l, PersistentP (x.2 κ tid l)) ∧
+    (∀ tid vl, (later_car (x.1.2 tid vl) : iProp Σ) -∗ ⌜length vl = x.1.1⌝) ∧
+    (∀ E κ l tid q, lftE ⊆ E →
+      lft_ctx -∗ &{κ} (l ↦∗: λ vs, later_car (x.1.2 tid vs)) -∗
+      q.[κ] ={E}=∗ x.2 κ tid l ∗ q.[κ]) ∧
+    (∀ κ κ' tid l, lft_ctx -∗ κ' ⊑ κ -∗ x.2 κ tid l -∗ x.2 κ' tid l).
 
-    Definition type_ofe_mixin : OfeMixin type.
-    Proof.
-      split; [|split|]; unfold equiv, dist, type_equiv, type_dist.
-      - intros. apply equiv_dist.
-      - by intros ?.
-      - by intros ???.
-      - by intros ???->.
-      - by intros ????; apply dist_S.
-    Qed.
+  Definition type_unpack (ty : type) : T :=
+    (ty.(ty_size), λ tid vl, Next (ty.(ty_own) tid vl), ty.(ty_shr)).
+  Program Definition type_pack (x : T) (H : P x) : type :=
+    {| ty_size := x.1.1; ty_own tid vl := later_car (x.1.2 tid vl); ty_shr := x.2 |}.
+  Solve Obligations with by intros [[??] ?] (?&?&?&?).
 
-    Canonical Structure typeC : ofeT := OfeT type type_ofe_mixin.
+  Definition type_ofe_mixin : OfeMixin type.
+  Proof.
+    apply (iso_ofe_mixin type_unpack).
+    - split; [by destruct 1|by intros [[??] ?]; constructor].
+    - split; [by destruct 1|by intros [[??] ?]; constructor].
+  Qed.
+  Canonical Structure typeC : ofeT := OfeT type type_ofe_mixin.
 
-    Instance st_equiv : Equiv simple_type := λ st1 st2,
-      @Next (_ -c> _ -c> _) st1.(st_own) ≡ @Next (_ -c> _ -c> _) st2.(st_own).
-    Instance st_dist : Dist simple_type := λ n st1 st2,
-      @Next (_ -c> _ -c> _) st1.(st_own) ≡{n}≡ @Next (_ -c> _ -c> _) st2.(st_own).
-
-    Definition st_ofe_mixin : OfeMixin simple_type.
-    Proof.
-      split; [|split|]; unfold equiv, dist, st_equiv, st_dist.
-      - intros. apply equiv_dist.
-      - by intros ?.
-      - by intros ???.
-      - by intros ???->.
-      - by intros ????; apply dist_S.
-    Qed.
-
-    Canonical Structure simple_typeC : ofeT := OfeT simple_type st_ofe_mixin.
-  End def.
-
-  Lemma st_dist_unfold n (x y : simple_type) :
-    x ≡{n}≡ y ↔
-      @Next (_ -c> _ -c> _) x.(st_own) ≡{n}≡ @Next (_ -c> _ -c> _) y.(st_own).
-  Proof. done. Qed.
-
-  Global Instance ty_size_proper_d n:
-    Proper (dist n ==> eq) ty_size.
+  Global Instance ty_size_ne n : Proper (dist n ==> eq) ty_size.
   Proof. intros ?? EQ. apply EQ. Qed.
-  Global Instance ty_size_proper_e :
-    Proper ((≡) ==> eq) ty_size.
+  Global Instance ty_size_proper : Proper ((≡) ==> eq) ty_size.
   Proof. intros ?? EQ. apply EQ. Qed.
   Global Instance ty_own_ne n:
     Proper (dist (S n) ==> eq ==> eq ==> dist n) ty_own.
   Proof. intros ?? EQ ??-> ??->. apply EQ. Qed.
-  Global Instance ty_own_proper_e:
-    Proper ((≡) ==> eq ==> eq ==> (≡)) ty_own.
+  Global Instance ty_own_proper : Proper ((≡) ==> eq ==> eq ==> (≡)) ty_own.
   Proof. intros ?? EQ ??-> ??->. apply EQ. Qed.
-  Global Instance ty_shr_ne n:
+  Global Instance ty_shr_ne n :
     Proper (dist n ==> eq ==> eq ==> eq ==> dist n) ty_shr.
   Proof. intros ?? EQ ??-> ??-> ??->. apply EQ. Qed.
-  Global Instance ty_shr_proper_e :
+  Global Instance ty_shr_proper :
     Proper ((≡) ==> eq ==> eq ==> eq ==> (≡)) ty_shr.
   Proof. intros ?? EQ ??-> ??-> ??->. apply EQ. Qed.
-  Global Instance st_own_ne n:
+
+  Global Instance type_cofe : Cofe typeC.
+  Proof.
+    apply: (iso_cofe_subtype P type_pack type_unpack).
+    - split; [by destruct 1|by intros [[??] ?]; constructor].
+    - by intros [].
+    - intros ? c. rewrite /P /=. split_and!.
+      + intros κ tid l. apply uPred.entails_equiv_and, equiv_dist=>n.
+        setoid_rewrite conv_compl; simpl.
+        apply equiv_dist, uPred.entails_equiv_and, ty_shr_persistent.
+      + intros tid vl. apply uPred.entails_equiv_and, equiv_dist=>n.
+        rewrite !conv_compl /=.
+        apply equiv_dist, uPred.entails_equiv_and, ty_size_eq.
+      + intros E κ l tid q ?. apply uPred.entails_equiv_and, equiv_dist=>n.
+        setoid_rewrite conv_compl; simpl.
+        rewrite -(c.(chain_cauchy) n (S n)); last lia.
+        by apply equiv_dist, uPred.entails_equiv_and, ty_share.
+      + intros κ κ' tid l. apply uPred.entails_equiv_and, equiv_dist=>n.
+        setoid_rewrite conv_compl; simpl.
+        apply equiv_dist, uPred.entails_equiv_and, ty_shr_mono.
+  Qed.
+
+  Inductive st_equiv' (ty1 ty2 : simple_type) : Prop :=
+    St_equiv :
+      (∀ tid vs, ty1.(ty_own) tid vs ≡ ty2.(ty_own) tid vs) →
+      st_equiv' ty1 ty2.
+  Instance st_equiv : Equiv simple_type := st_equiv'.
+  Inductive st_dist' (n : nat) (ty1 ty2 : simple_type) : Prop :=
+    St_dist :
+      (∀ tid vs, dist_later n (ty1.(ty_own) tid vs) (ty2.(ty_own) tid vs)) →
+      st_dist' n ty1 ty2.
+  Instance st_dist : Dist simple_type := st_dist'.
+
+  Definition st_unpack (ty : simple_type) : thread_id -c> list val -c> laterC (iProp Σ) :=
+    λ tid vl, Next (ty.(ty_own) tid vl).
+
+  Definition st_ofe_mixin : OfeMixin simple_type.
+  Proof.
+    apply (iso_ofe_mixin st_unpack).
+    - split; [by destruct 1|by constructor].
+    - split; [by destruct 1|by constructor].
+  Qed.
+  Canonical Structure stC : ofeT := OfeT simple_type st_ofe_mixin.
+
+  Global Instance st_own_ne n :
     Proper (dist (S n) ==> eq ==> eq ==> dist n) st_own.
   Proof. intros ?? EQ ??-> ??->. apply EQ. Qed.
-  Global Instance st_own_proper_e :
-    Proper ((≡) ==> eq ==> eq ==> (≡)) st_own.
+  Global Instance st_own_proper : Proper ((≡) ==> eq ==> eq ==> (≡)) st_own.
   Proof. intros ?? EQ ??-> ??->. apply EQ. Qed.
 
-  Global Program Instance type_cofe : Cofe typeC :=
-    {| compl c :=
-         let '(ty_size, Next ty_own, ty_shr) :=
-             compl {| chain_car := tuple_of_type ∘ c |}
-         in
-         {| ty_size := ty_size; ty_own := ty_own; ty_shr := ty_shr |}
-    |}.
-  Next Obligation. intros [c Hc]. apply Hc. Qed.
-  Next Obligation.
-    simpl. intros c _ _ shr [=_ _ ->] κ tid l.
-    apply uPred.equiv_entails, equiv_dist=>n.
-    by rewrite (λ c, conv_compl (A:=_ -c> _ -c> _ -c> _) n c κ tid l) /=
-               uPred.always_always.
-  Qed.
-  Next Obligation.
-    simpl. intros c sz own _ [=-> -> _] tid vl.
-    apply uPred.entails_equiv_and, equiv_dist=>n.
-    rewrite (λ c, conv_compl (A:=_ -c> _ -c> _) n c tid vl) /= conv_compl /=.
-    apply equiv_dist, uPred.entails_equiv_and, ty_size_eq.
-  Qed.
-  Next Obligation.
-    simpl. intros c _ own shr [=_ -> ->] E κ l tid q ?.
-    apply uPred.entails_equiv_and, equiv_dist=>n.
-    rewrite (λ c, conv_compl (A:=_ -c> _ -c> _ -c> _) n c κ tid l) /=.
-    setoid_rewrite (λ c vl, conv_compl (A:=_ -c> _ -c> _) n c tid vl). simpl.
-    etrans. { by apply equiv_dist, uPred.entails_equiv_and, (c n).(ty_share). }
-    simpl. destruct n; repeat (simpl; (f_contractive || f_equiv)).
-    rewrite (c.(chain_cauchy) (S n) (S (S n))) //. lia.
-  Qed.
-  Next Obligation.
-    simpl. intros c _ _ shr [=_ _ ->] κ κ' tid l.
-    apply uPred.entails_equiv_and, equiv_dist=>n.
-    rewrite !(λ c, conv_compl (A:=_ -c> _ -c> _ -c> _) n c _ tid l) /=.
-    apply equiv_dist, uPred.entails_equiv_and. apply ty_shr_mono.
-  Qed.
-  Next Obligation.
-    intros n c. split; [split|]; simpl; try by rewrite conv_compl.
-    set (c n). f_contractive. rewrite conv_compl //.
-  Qed.
-
-  Global Instance ty_of_st_ne n : Proper (dist n ==> dist n) ty_of_st.
+  Global Instance ty_of_st_ne : NonExpansive ty_of_st.
   Proof.
-    intros [][]EQ. split;[split|]=>//= κ tid l.
-    repeat (f_contractive || f_equiv). apply EQ.
+    intros n ?? EQ. constructor. done. simpl.
+    - intros tid l. apply EQ.
+    - simpl. intros; repeat (f_contractive || f_equiv). apply EQ.
   Qed.
+  Global Instance ty_of_st_proper : Proper ((≡) ==> (≡)) ty_of_st.
+  Proof. apply (ne_proper _). Qed.
 End ofe.
 
 Section subtyping.
@@ -382,16 +376,16 @@ Section subtyping.
   Lemma equiv_subtype ty1 ty2 : ty1 ≡ ty2 → subtype ty1 ty2.
   Proof. unfold subtype, type_incl=>EQ. setoid_rewrite EQ. apply subtype_refl. Qed.
 
-  Global Instance ty_size_proper : Proper (subtype ==> ctx_eq) ty_size.
+  Global Instance ty_size_subtype : Proper (subtype ==> ctx_eq) ty_size.
   Proof. iIntros (?? Hst) "LFT HE HL". iDestruct (Hst with "LFT HE HL") as "[$ ?]". Qed.
-  Global Instance ty_size_proper_flip : Proper (flip subtype ==> ctx_eq) ty_size.
+  Global Instance ty_size_subtype_flip : Proper (flip subtype ==> ctx_eq) ty_size.
   Proof. by intros ?? ->. Qed.
-  Lemma ty_size_proper' ty1 ty2 :
+  Lemma ty_size_subtype' ty1 ty2 :
     subtype ty1 ty2 → ctx_eq (ty_size ty1) (ty_size ty2).
-  Proof. apply ty_size_proper. Qed.
-  Lemma ty_size_proper_flip' ty1 ty2 :
+  Proof. apply ty_size_subtype. Qed.
+  Lemma ty_size_subtype_flip' ty1 ty2 :
     subtype ty2 ty1 → ctx_eq (ty_size ty1) (ty_size ty2).
-  Proof. apply ty_size_proper_flip. Qed.
+  Proof. apply ty_size_subtype_flip. Qed.
 
   (* TODO: The prelude should have a symmetric closure. *)
   Definition eqtype (ty1 ty2 : type) : Prop :=
@@ -471,6 +465,6 @@ Section weakening.
   Qed.
 End weakening.
 
-Hint Resolve subtype_refl eqtype_refl ctx_eq_refl ty_size_proper'
-             ty_size_proper_flip': lrust_typing.
+Hint Resolve subtype_refl eqtype_refl ctx_eq_refl ty_size_subtype'
+             ty_size_subtype_flip': lrust_typing.
 Hint Opaque ctx_eq subtype eqtype : lrust_typing.
